[Dafny] Start proving compile_def

compiler/dafny/dafny_compilerScript.sml
@@ -13,14 +13,25 @@ open simpleSexpParseTheory
 
 val _ = new_theory "dafny_compiler";
 
-Definition dfy_to_cml_def:
-  dfy_to_cml (dfy_sexp: string) =
+(* Trusted frontend *)
+Definition frontend_def:
+  frontend (dfy_sexp: string) =
   do
     dfy_sexp <- lex dfy_sexp;
     dfy_sexp <- parse dfy_sexp;
-    dfy <- to_program dfy_sexp;
-    dfy <<- freshen_program dfy;
-    from_program dfy
+    to_program dfy_sexp
+  od
+End
+
+Definition compile_def:
+  compile dfy = from_program (freshen_program dfy)
+End
+
+Definition dfy_to_cml_def:
+  dfy_to_cml (dfy_sexp: string) =
+  do
+    dfy <- frontend dfy_sexp;
+    compile dfy
   od
 End
 
