compiler/dafny/semantics/dafny_compilerProofScript.sml
@@ -1,0 +1,155 @@
+(*
+  Correctness proof for the Dafny compiler with all of its passes.
+*)
+
+open preamble
+open dafny_semanticPrimitivesTheory
+open dafny_freshenTheory
+open dafny_freshenProofTheory
+open dafny_to_cakemlTheory
+open dafny_to_cakemlProofTheory
+open dafny_compilerTheory
+open mlstringTheory  (* isPrefix *)
+
+val _ = new_theory "dafny_compilerProof";
+val _ = set_grammar_ancestry
+          ["dafny_semanticPrimitives", "dafny_freshen", "dafny_freshenProof",
+           "dafny_to_cakeml", "dafny_to_cakemlProof", "dafny_compiler",
+           "mlstring"];
+
+(* TODO Upstream? *)
+Triviality UNZIP_LENGTH:
+  ∀xs ys zs. UNZIP xs = (ys, zs) ⇒ LENGTH ys = LENGTH zs
+Proof
+  Induct \\ gvs []
+QED
+
+(* TODO Upstream? *)
+Triviality UNZIP_EQ_NIL:
+  (UNZIP l = (xs, []) ⇔ l = [] ∧ xs = []) ∧
+  (UNZIP l = ([], ys) ⇔ l = [] ∧ ys = [])
+Proof
+  Cases_on ‘l’ \\ gvs []
+QED
+
+(* by magnus *)
+Theorem exists_mlstring:
+  (∃x:mlstring. P x) ⇔ (∃s. P (strlit s))
+Proof
+  eq_tac \\ rw []
+  >- (Cases_on ‘x’ \\ gvs [] \\ pop_assum $ irule_at Any)
+  \\ pop_assum $ irule_at Any
+QED
+
+Theorem isprefix_strcat:
+  ∀s₁ s₂. isPrefix s₁ s₂ = ∃s₃. s₂ = s₁ ^ s₃
+Proof
+  rpt gen_tac
+  \\ gvs [isprefix_thm, strcat_thm, isPREFIX_STRCAT, exists_mlstring,
+          implode_def]
+  \\ Cases_on ‘s₂’ \\ simp []
+QED
+
+(* TODO Move is_fresh properties to to separate file? *)
+
+(* ** *)
+(* TODO Already exists in freshenProof; make it Theorem *)
+Triviality map_add_fresh_exists:
+  ∀m cnt ns cnt' m'.
+    map_add_fresh m cnt ns = (cnt', m') ⇒
+    ∃m₁. m' = m₁ ++ m ∧ MAP FST m₁ = REVERSE ns
+Proof
+  Induct_on ‘ns’ \\ rpt strip_tac
+  \\ gvs [map_add_fresh_def, add_fresh_def]
+  \\ last_x_assum drule_all \\ rpt strip_tac \\ gvs []
+QED
+
+Triviality lookup_append_eq:
+  ∀n m₁ m₀.
+    MEM n (MAP FST m₁) ⇒ lookup (m₁ ++ m₀) n = lookup m₁ n
+Proof
+  rpt strip_tac
+  \\ gvs [lookup_def, ALOOKUP_APPEND]
+  \\ Cases_on ‘ALOOKUP m₁ n’
+  \\ gvs [ALOOKUP_NONE]
+QED
+(* ** *)
+
+Triviality map_add_fresh_every_is_fresh:
+  ∀ns m cnt cnt' m'.
+    map_add_fresh m cnt ns = (cnt', m') ∧
+    ALL_DISTINCT ns ⇒
+    EVERY (λn. is_fresh n) (MAP (lookup m') ns)
+Proof
+  Induct \\ simp []
+  \\ qx_gen_tac ‘n’ \\ rpt strip_tac
+  >-
+   (drule map_add_fresh_exists
+    \\ rpt strip_tac \\ gvs []
+    \\ ‘MEM n (MAP FST m₁)’ by gvs []
+    \\ drule lookup_append_eq \\ simp []
+    \\ disch_then kall_tac
+    \\ simp [lookup_def]
+    \\ CASE_TAC
+    >- (gvs [ALOOKUP_NONE])
+    \\ simp [is_fresh_def, isprefix_strcat])
+  \\ gvs [map_add_fresh_def, add_fresh_def]
+  \\ last_assum irule
+  \\ last_assum $ irule_at Any
+QED
+
+Triviality freshen_member_is_fresh:
+  freshen_member member = fresh_member ⇒ is_fresh_member fresh_member
+Proof
+  disch_tac
+  \\ Cases_on ‘member’
+  \\ gvs [freshen_member_def]
+  \\ rpt (pairarg_tac \\ gvs [])
+  >-
+   (imp_res_tac UNZIP_LENGTH
+    \\ simp [MAP_ZIP]
+QED
+
+(* *** *)
+
+Triviality has_main_freshen:
+  has_main (Program (MAP freshen_member members)) =
+  has_main (Program members)
+Proof
+  Induct_on ‘members’ \\ simp []
+  \\ qx_gen_tac ‘member’
+  \\ gvs [has_main_def, get_member_def, get_member_aux_def]
+  \\ Cases_on ‘member’ \\ simp [freshen_member_def]
+  \\ rpt (pairarg_tac \\ gvs [])
+  \\ imp_res_tac UNZIP_LENGTH
+  \\ IF_CASES_TAC \\ gvs []
+  \\ eq_tac
+  \\ rpt strip_tac
+  \\ gvs [ZIP_EQ_NIL, UNZIP_EQ_NIL]
+QED
+
+Theorem correct_compile:
+  ∀dfy_ck prog s' r_dfy cml_decs env_cml (t: 'ffi cml_state).
+    evaluate_program dfy_ck T prog = (s', r_dfy) ∧
+    compile prog = INR cml_decs ∧
+    has_main prog ∧ has_basic_cons env_cml ∧
+    0 < dfy_ck ∧ t.clock = dfy_ck ∧ ExnStamp t.next_exn_stamp = ret_stamp ∧
+    r_dfy ≠ Rstop (Serr Rtype_error) ⇒
+    ∃ck t' m' r_cml.
+      evaluate_decs (t with clock := t.clock + ck) env_cml cml_decs =
+        (t', r_cml) ∧
+      state_rel m' FEMPTY s' t' env_cml ∧ stmt_res_rel r_dfy r_cml
+Proof
+  rpt strip_tac
+  \\ irule correct_from_program
+  \\ fs [compile_def]
+  \\ last_assum $ irule_at (Pos last)
+  \\ irule_at (Pos last) correct_freshen_program \\ simp []
+  \\ namedCases_on ‘prog’ ["members"]
+  \\ simp [valid_prog_def, freshen_program_def, has_main_freshen]
+
+  \\ cheat
+QED
+
+
+val _ = export_theory ();
